wip, syntax refactoring

examples/dsls/mini_steel/Pulse.Checker.Bind.fst
@@ -14,24 +14,24 @@ module FV = Pulse.Typing.FV
 
 #push-options "--z3rlimit_factor 8 --ifuel 1 --fuel 2"
 let rec mk_bind (f:RT.fstar_top_env) (g:env)
-  (pre:pure_term)
-  (e1:term)
-  (e2:term)
-  (c1:pure_comp_st)
-  (c2:pure_comp_st)
+  (pre:term)
+  (e1:st_term)
+  (e2:st_term)
+  (c1:comp_st)
+  (c2:comp_st)
   (x:var)
-  (d_e1:src_typing f g e1 c1)
+  (d_e1:st_typing f g e1 c1)
   (d_c1res:tot_typing f g (comp_res c1) (Tm_Type (comp_u c1)))
-  (d_e2:src_typing f ((x, Inl (comp_res c1))::g) (open_term e2 x) c2)
+  (d_e2:st_typing f ((x, Inl (comp_res c1))::g) (open_st_term e2 x) c2)
   (res_typing:universe_of f g (comp_res c2) (comp_u c2))
   (post_typing:tot_typing f ((x, Inl (comp_res c2))::g) (open_term (comp_post c2) x) Tm_VProp)
-  : T.TacH (t:term &
-            c:pure_comp { stateful_comp c ==> comp_pre c == pre } &
-            src_typing f g t c)
+  : T.TacH (t:st_term &
+            c:comp { stateful_comp c ==> comp_pre c == pre } &
+            st_typing f g t c)
            (requires fun _ ->
               comp_pre c1 == pre /\
               None? (lookup g x) /\
-              (~(x `Set.mem` freevars e2)) /\
+              (~(x `Set.mem` freevars_st e2)) /\
               open_term (comp_post c1) x == comp_pre c2 /\
               (~ (x `Set.mem` freevars (comp_post c2))))
            (ensures fun _ _ -> True) =
@@ -53,7 +53,7 @@ let rec mk_bind (f:RT.fstar_top_env) (g:env)
     then begin
       assume (inames == Tm_EmpInames);
       let c1lifted = C_ST (st_comp_of_comp c1) in
-      let d_e1 : src_typing f g e1 c1lifted =
+      let d_e1 : st_typing f g e1 c1lifted =
         T_Lift _ _ _ c1lifted d_e1 (Lift_STAtomic_ST _ c1) in
       let bc = Bind_comp g x c1lifted c2 res_typing x post_typing in
       (| Tm_Bind e1 e2, _, T_Bind _ e1 e2 _ _ _ _ d_e1 d_c1res d_e2 bc |)
@@ -83,7 +83,7 @@ let rec mk_bind (f:RT.fstar_top_env) (g:env)
       assume (inames == Tm_EmpInames);
       let c2lifted = C_ST (st_comp_of_comp c2) in
       let g' = (x, Inl (comp_res c1))::g in
-      let d_e2 : src_typing f g' (open_term e2 x) c2lifted =
+      let d_e2 : st_typing f g' (open_st_term e2 x) c2lifted =
         T_Lift _ _ _ c2lifted d_e2 (Lift_STAtomic_ST _ c2) in
       let bc = Bind_comp g x c1 c2lifted res_typing x post_typing in
       (| Tm_Bind e1 e2, _, T_Bind _ e1 e2 _ _ _ _ d_e1 d_c1res d_e2 bc |)
@@ -95,7 +95,7 @@ let rec mk_bind (f:RT.fstar_top_env) (g:env)
       assume (inames == Tm_EmpInames);
       let w = get_non_informative_witness f g (comp_u c1) (comp_res c1) in
       let c1lifted = C_STAtomic inames (st_comp_of_comp c1) in
-      let d_e1 : src_typing f g e1 c1lifted =
+      let d_e1 : st_typing f g e1 c1lifted =
         T_Lift _ _ _ c1lifted d_e1 (Lift_STGhost_STAtomic g c1 w) in
       mk_bind f g pre e1 e2 c1lifted c2 x d_e1 d_c1res d_e2 res_typing post_typing
     end
@@ -107,7 +107,7 @@ let rec mk_bind (f:RT.fstar_top_env) (g:env)
       let g' = (x, Inl (comp_res c1))::g in
       let w = get_non_informative_witness f g' (comp_u c2) (comp_res c2) in
       let c2lifted = C_STAtomic inames (st_comp_of_comp c2) in
-      let d_e2 : src_typing f g' (open_term e2 x) c2lifted =
+      let d_e2 : st_typing f g' (open_st_term e2 x) c2lifted =
         T_Lift _ _ _ c2lifted d_e2 (Lift_STGhost_STAtomic g' c2 w) in
       mk_bind f g pre e1 e2 c1 c2lifted x d_e1 d_c1res d_e2 res_typing post_typing
     end
@@ -117,7 +117,7 @@ let rec mk_bind (f:RT.fstar_top_env) (g:env)
     then begin
       assume (inames == Tm_EmpInames);
       let c1lifted = C_ST (st_comp_of_comp c1) in
-      let d_e1 : src_typing f g e1 c1lifted =
+      let d_e1 : st_typing f g e1 c1lifted =
         T_Lift _ _ _ c1lifted d_e1 (Lift_STAtomic_ST _ c1) in
       mk_bind f g pre e1 e2 c1lifted c2 x d_e1 d_c1res d_e2 res_typing post_typing
     end
@@ -129,14 +129,14 @@ let rec mk_bind (f:RT.fstar_top_env) (g:env)
 let check_bind
   (f:RT.fstar_top_env)
   (g:env)
-  (t:term{Tm_Bind? t})
-  (pre:pure_term)
+  (t:st_term{Tm_Bind? t})
+  (pre:term)
   (pre_typing:tot_typing f g pre Tm_VProp)
   (post_hint:option term)
   (check:check_t)
-  : T.Tac (t:term &
-           c:pure_comp { stateful_comp c ==> comp_pre c == pre } &
-           src_typing f g t c) =
+  : T.Tac (t:st_term &
+           c:comp { stateful_comp c ==> comp_pre c == pre } &
+           st_typing f g t c) =
   let Tm_Bind e1 e2 = t  in
   let (| e1, c1, d1 |) = check f g e1 pre pre_typing None in
   let (| c1, d1 |) = force_st pre_typing (| c1, d1 |) in
@@ -158,13 +158,13 @@ let check_bind
       let next_pre_typing : tot_typing f g' next_pre Tm_VProp
         = check_vprop_no_inst f g' next_pre
       in
-      let (| e2', c2, d2 |) = check f g' (open_term e2 x) next_pre next_pre_typing post_hint in
-      FV.src_typing_freevars d2;
+      let (| e2', c2, d2 |) = check f g' (open_st_term e2 x) next_pre next_pre_typing post_hint in
+      FV.st_typing_freevars d2;
       let (| c2, d2 |) = force_st #_ #_ #e2' next_pre_typing (| c2, d2 |) in
-      let e2_closed = close_term e2' x in
-      assume (open_term e2_closed x == e2');
-      let d2 : src_typing f g' e2' c2 = d2 in
-      let d2 : src_typing f g' (open_term e2_closed x) c2 = d2 in
+      let e2_closed = close_st_term e2' x in
+      assume (open_st_term e2_closed x == e2');
+      let d2 : st_typing f g' e2' c2 = d2 in
+      let d2 : st_typing f g' (open_st_term e2_closed x) c2 = d2 in
       let s2 = st_comp_of_comp c2 in
       let (| u, res_typing |) = check_universe f g s2.res in
       if u <> s2.u
@@ -174,6 +174,7 @@ let check_bind
       else (
         let s2_post_opened = open_term s2.post x in
         let post_typing = check_vprop_no_inst f ((x, Inl s2.res)::g) s2_post_opened in
+        //assume (~ (x `Set.mem` freevars_st e2_closed));
         mk_bind f g pre e1 e2_closed c1 c2 x d1 t_typing d2 res_typing post_typing
       )
   )
